examples/pseudo_bool/array/npbc_parseProgScript.sml
@@ -1266,4 +1266,258 @@ Proof
   metis_tac[STDIO_INSTREAM_LINES_refl,STDIO_INSTREAM_LINES_ARRAY_refl]
 QED
 
+val r = translate parse_header_line_fast_def;
+
+Definition check_f_line_def:
+  (check_f_line [] = F) ∧
+  (check_f_line ((s: mlstring + int)::ss) ⇔ s = INL (strlit "f"))
+End
+
+val r = translate check_f_line_def;
+
+Definition check_header_full_def:
+  check_header_full s s' =
+  case s of NONE => SOME 0
+  | SOME s =>
+  case s' of NONE => SOME 1
+  | SOME s' =>
+  if parse_header_line_fast s then
+    if check_f_line s' then NONE
+    else SOME (1:num)
+  else SOME 0
+End
+
+val r = translate check_header_full_def;
+
+val check_header = process_topdecs`
+  fun check_header fd =
+  let
+    val s1 = TextIO.b_inputLineTokens fd blanks tokenize_fast
+    val s2 = TextIO.b_inputLineTokens fd blanks tokenize_fast
+  in
+  check_header_full s1 s2
+  end` |> append_prog;
+
+val b_inputLineTokens_specialize =
+  b_inputLineTokens_spec_lines
+  |> Q.GEN `f` |> Q.SPEC`blanks`
+  |> Q.GEN `fv` |> Q.SPEC`blanks_v`
+  |> Q.GEN `g` |> Q.ISPEC`tokenize_fast`
+  |> Q.GEN `gv` |> Q.ISPEC`tokenize_fast_v`
+  |> Q.GEN `a` |> Q.ISPEC`SUM_TYPE STRING_TYPE INT`
+  |> SIMP_RULE std_ss [blanks_v_thm,tokenize_fast_v_thm,blanks_def] ;
+
+Theorem check_header_spec:
+  !ss fd fdv lines fs.
+  app (p : 'ffi ffi_proj)
+    ^(fetch_v "check_header" (get_ml_prog_state()))
+    [fdv]
+    (STDIO fs * INSTREAM_LINES fd fdv lines fs)
+    (POSTv v.
+       SEP_EXISTS k lines' res.
+       STDIO (forwardFD fs fd k) *
+       INSTREAM_LINES fd fdv lines' (forwardFD fs fd k) *
+       &(OPTION_TYPE NUM res v))
+Proof
+  xcf "check_header" (get_ml_prog_state ())>>
+  rpt xlet_autop>>
+  xlet ‘(POSTv v.
+      SEP_EXISTS k.
+          STDIO (forwardFD fs fd k) *
+          INSTREAM_LINES fd fdv (TL lines) (forwardFD fs fd k) *
+          &OPTION_TYPE (LIST_TYPE (SUM_TYPE STRING_TYPE INT))
+            (OPTION_MAP (MAP tokenize_fast ∘ tokens blanks) (oHD lines)) v)’
+  >- (
+    xapp_spec b_inputLineTokens_specialize
+    \\ qexists_tac ‘emp’
+    \\ xsimpl)>>
+  xlet ‘(POSTv v.
+      SEP_EXISTS k.
+          STDIO (forwardFD fs fd k) *
+          INSTREAM_LINES fd fdv (TL (TL lines)) (forwardFD fs fd k) *
+          &OPTION_TYPE (LIST_TYPE (SUM_TYPE STRING_TYPE INT))
+            (OPTION_MAP (MAP tokenize_fast ∘ tokens blanks) (oHD (TL lines))) v)’
+  >- (
+    xapp_spec b_inputLineTokens_specialize
+    \\ qexists_tac ‘emp’
+    \\ xsimpl
+    \\ metis_tac[forwardFD_o,STDIO_INSTREAM_LINES_refl,STDIO_INSTREAM_LINES_refl_gc]
+    )>>
+  xapp>>
+  xsimpl>>
+  metis_tac[forwardFD_o,STDIO_INSTREAM_LINES_refl,STDIO_INSTREAM_LINES_refl_gc]
+QED
+
+Definition result_string_def:
+  result_string success_string ob =
+   case ob of
+    INR b =>
+      if b then INR success_string
+      else INL (strlit "Proof checking succeeded but did not derive contradiction\n")
+  | INL v => INL v
+End
+
+val r = translate result_string_def;
+
+Definition notfound_string_def:
+  notfound_string f = concat[strlit"c Input file: ";f;strlit" no such file or directory\n"]
+End
+
+val r = translate notfound_string_def;
+
+val check_unsat_top = process_topdecs `
+  fun check_unsat_top success_string fml fname =
+  let
+    val fd = TextIO.b_openIn fname
+  in
+    case check_header fd of
+      Some n =>
+      (TextIO.b_closeIn fd;
+      Inl (format_failure n "Unable to parse header"))
+    | None =>
+      let val res =
+        result_string success_string (check_unsat fd 2 fml)
+        val close = TextIO.b_closeIn fd;
+      in
+        res
+      end
+  end
+  handle TextIO.BadFileName => Inl (notfound_string fname)` |> append_prog;
+
+Theorem STDIO_INSTREAM_LINES_refl_more_gc:
+  STDIO A *
+  INSTREAM_LINES B C D E * rest ==>>
+  STDIO A *
+  INSTREAM_LINES B C D E * GC
+Proof
+  xsimpl
+QED
+
+Theorem check_unsat_top_spec:
+  LIST_TYPE
+    (PAIR_TYPE PBC_PBOP_TYPE
+       (PAIR_TYPE (LIST_TYPE (PAIR_TYPE INT (PBC_LIT_TYPE STRING_TYPE)))
+          INT)) fml fmlv ∧
+  FILENAME f fv ∧
+  hasFreeFD fs ∧
+  STRING_TYPE success successv ∧
+  pbf_vars (set fml) ⊆ goodString
+  ⇒
+  app (p:'ffi ffi_proj) ^(fetch_v"check_unsat_top"(get_ml_prog_state()))
+  [successv; fmlv; fv]
+  (STDIO fs)
+  (POSTv v.
+     STDIO fs *
+     SEP_EXISTS res.
+     &(
+      SUM_TYPE STRING_TYPE STRING_TYPE res v ∧
+      (∀s. res = INR s ⇒
+        (s = success ∧
+        unsatisfiable (set fml)))))
+Proof
+  xcf"check_unsat_top"(get_ml_prog_state()) >>
+  reverse (Cases_on `STD_streams fs`)
+  >- (fs [TextIOProofTheory.STDIO_def] \\ xpull) >>
+  reverse (Cases_on`consistentFS fs`)
+  >- (fs [STDIO_def,IOFS_def,wfFS_def,consistentFS_def] \\ xpull \\ metis_tac[]) >>
+  reverse (Cases_on `inFS_fname fs f`) >> simp[]
+  >- (
+    xhandle`POSTe ev.
+      &BadFileName_exn ev *
+      &(~inFS_fname fs f) *
+      STDIO fs`
+    >-
+      (xlet_auto_spec (SOME b_openIn_STDIO_spec) \\ xsimpl)
+    >>
+      fs[BadFileName_exn_def]>>
+      xcases>>rw[]>>
+      xlet_auto>>xsimpl>>
+      xcon>>xsimpl>>
+      qexists_tac`INL (notfound_string f)`>>
+      simp[SUM_TYPE_def])>>
+  qmatch_goalsub_abbrev_tac`$POSTv Qval`>>
+  xhandle`$POSTv Qval` \\ xsimpl >>
+  qunabbrev_tac`Qval`>>
+  xlet_auto_spec (SOME b_openIn_spec_lines) \\ xsimpl >>
+  qmatch_goalsub_abbrev_tac`INSTREAM_LINES fd fdv lines fss`>>
+  xlet`POSTv v.
+    SEP_EXISTS k lines' res.
+    STDIO (forwardFD fss fd k) *
+    INSTREAM_LINES fd fdv lines' (forwardFD fss fd k) *
+    &OPTION_TYPE NUM res v`
+  >- (
+    xapp>>
+    qexists_tac`emp`>>
+    xsimpl>>
+    metis_tac[STDIO_INSTREAM_LINES_refl,STDIO_INSTREAM_LINES_refl_gc,STAR_COMM])>>
+  qmatch_goalsub_abbrev_tac`INSTREAM_LINES fd fdv _ fsss`>>
+  reverse (Cases_on`res`)>>fs[OPTION_TYPE_def]>>xmatch
+  >- (
+    xlet `POSTv v. STDIO fs`
+    >- (
+      xapp_spec b_closeIn_spec_lines >>
+      xsimpl>>
+      qexists_tac `emp`>>
+      qexists_tac `lines'` >>
+      qexists_tac `fsss`>>
+      qexists_tac `fd` >>
+      conj_tac THEN1
+        (unabbrev_all_tac
+        \\ imp_res_tac fsFFIPropsTheory.nextFD_ltX \\ fs []
+        \\ imp_res_tac fsFFIPropsTheory.STD_streams_nextFD \\ fs []) >>
+      xsimpl>>
+      `validFileFD fd fsss.infds` by
+        (unabbrev_all_tac>> simp[validFileFD_forwardFD]
+         \\ imp_res_tac fsFFIPropsTheory.nextFD_ltX \\ fs []
+         \\ match_mp_tac validFileFD_nextFD \\ fs []) >>
+      xsimpl >> rw [] >>
+      unabbrev_all_tac>>xsimpl>>
+      simp[forwardFD_ADELKEY_same]>>
+      DEP_REWRITE_TAC [fsFFIPropsTheory.openFileFS_ADELKEY_nextFD]>>
+      xsimpl>>
+      imp_res_tac (DECIDE ``n<m:num ==> n <= m``) >>
+      imp_res_tac fsFFIPropsTheory.nextFD_leX \\ fs [])>>
+    xlet_autop>>
+    xcon>>
+    xsimpl>>
+    metis_tac[SUM_TYPE_def,sum_distinct])>>
+  xlet`POSTv v. SEP_EXISTS k lines' lno' fmlv' fmllsv' res.
+          STDIO (forwardFD fsss fd k) *
+          INSTREAM_LINES fd fdv lines' (forwardFD fsss fd k) *
+          &(SUM_TYPE STRING_TYPE BOOL res v ∧
+           (res = INR T ⇒ unsatisfiable (set fml)))`
+  >- (
+    xapp>>xsimpl>>
+    qexists_tac`emp`>>xsimpl>>
+    metis_tac[STDIO_INSTREAM_LINES_refl_more_gc,STDIO_INSTREAM_LINES_refl])>>
+  xlet_autop>>
+  xlet `POSTv v. STDIO fs`
+  >- (
+    xapp_spec b_closeIn_spec_lines >>
+    xsimpl>>
+    qexists_tac `emp`>>
+    qexists_tac `lines'` >>
+    qexists_tac `forwardFD fsss fd k'`>>
+    qexists_tac `fd` >>
+    conj_tac THEN1
+      (unabbrev_all_tac
+      \\ imp_res_tac fsFFIPropsTheory.nextFD_ltX \\ fs []
+      \\ imp_res_tac fsFFIPropsTheory.STD_streams_nextFD \\ fs []) >>
+    xsimpl>>
+    `validFileFD fd (forwardFD fsss fd k').infds` by
+      (unabbrev_all_tac>> simp[validFileFD_forwardFD]
+       \\ imp_res_tac fsFFIPropsTheory.nextFD_ltX \\ fs []
+       \\ match_mp_tac validFileFD_nextFD \\ fs []) >>
+    xsimpl >> rw [] >>
+    unabbrev_all_tac>>xsimpl>>
+    simp[forwardFD_ADELKEY_same]>>
+    DEP_REWRITE_TAC [fsFFIPropsTheory.openFileFS_ADELKEY_nextFD]>>
+    xsimpl>>
+    imp_res_tac (DECIDE ``n<m:num ==> n <= m``) >>
+    imp_res_tac fsFFIPropsTheory.nextFD_leX \\ fs [])>>
+  xvar>>xsimpl>>
+  asm_exists_tac>>fs[]>>
+  Cases_on`res`>>gs[result_string_def]
+QED
+
 val _ = export_theory();
