examples/pseudo_bool/array/subgraph_isoProgScript.sml
@@ -8,11 +8,7 @@ val _ = new_theory "subgraph_isoProg";
 
 val _ = translation_extends "npbc_parseProg";
 
-Definition usage_string_def:
-  usage_string = strlit "Usage: subgraph_iso_encode <LAD format file (pattern)> <LAD format file (target)> <proof (optional)>\n"
-End
-
-val r = translate usage_string_def;
+val xlet_autop = xlet_auto >- (TRY( xcon) >> xsimpl)
 
 Definition notfound_string_def:
   notfound_string f = concat[strlit"c Input file: ";f;strlit" no such file or directory\n"]
@@ -25,17 +21,16 @@ val noparse_string_def = Define`
 
 val r = translate noparse_string_def;
 
-val _ = translate graph_basicTheory.tokenize_def;
+val _ = translate mlintTheory.fromNatString_def;
+val _ = translate tokenize_num_def;
 
 val _ = translate parse_num_list_def;
-val _ = translate insert_def;
 val _ = translate parse_edges_def;
 val _ = translate parse_lad_toks_def;
 
 val _ = translate lrnext_def;
 val _ = translate foldi_def;
 val _ = translate toAList_def;
-val _ = translate lookup_def;
 
 Theorem check_good_edges_inner_thm:
   check_good_edges_inner u v es ⇔
@@ -52,7 +47,7 @@ val _ = translate check_good_graph_def;
 
 val parse_lad = (append_prog o process_topdecs) `
   fun parse_lad f =
-  (case TextIO.b_inputAllTokensFrom f blanks tokenize of
+  (case TextIO.b_inputAllTokensFrom f blanks tokenize_num of
     None => Inl (notfound_string f)
   | Some lines =>
   (case parse_lad_toks lines of
@@ -60,7 +55,98 @@ val parse_lad = (append_prog o process_topdecs) `
   | Some x =>
     if check_good_graph x then
       Inr x
-    else Inl ("c WARNING: Input graph file (" ^ f ^ ") fails undirectedness check\n")))`
+    else Inl ("Input graph file (" ^ f ^ ") fails undirectedness check\n")))`
+
+val tokenize_num_v_thm = theorem "tokenize_num_v_thm";
+
+val b_inputAllTokensFrom_spec_specialize =
+  b_inputAllTokensFrom_spec
+  |> Q.GEN `f` |> Q.SPEC`blanks`
+  |> Q.GEN `fv` |> Q.SPEC`blanks_v`
+  |> Q.GEN `g` |> Q.ISPEC`graph_basic$tokenize_num`
+  |> Q.GEN `gv` |> Q.ISPEC`tokenize_num_v`
+  |> Q.GEN `a` |> Q.ISPEC`SUM_TYPE STRING_TYPE NUM`
+  |> REWRITE_RULE [blanks_v_thm,tokenize_num_v_thm] ;
+
+Definition get_graph_def:
+  get_graph fs f =
+  if inFS_fname fs f then
+    (case parse_lad (all_lines fs f) of
+      NONE => NONE
+    | SOME x =>
+      if check_good_graph x then SOME x
+      else NONE)
+  else NONE
+End
+
+Theorem parse_lad_spec:
+  STRING_TYPE f fv ∧
+  validArg f ∧
+  hasFreeFD fs
+  ⇒
+  app (p:'ffi ffi_proj) ^(fetch_v"parse_lad"(get_ml_prog_state()))
+    [fv]
+    (STDIO fs)
+    (POSTv v.
+    & (∃res.
+      SUM_TYPE STRING_TYPE (PAIR_TYPE NUM (SPTREE_SPT_TYPE (LIST_TYPE NUM))) res v ∧
+      case res of
+        INR g => get_graph fs f = SOME g
+      | INL err => get_graph fs f = NONE
+      )
+      * STDIO fs)
+Proof
+  rw[]>>
+  xcf"parse_lad"(get_ml_prog_state())>>
+  reverse (Cases_on `STD_streams fs`) >- (fs [TextIOProofTheory.STDIO_def] \\ xpull) >>
+  reverse (Cases_on`consistentFS fs`) >- (
+    fs [STDIO_def,IOFS_def,wfFS_def,consistentFS_def]
+    \\ xpull \\ metis_tac[]) >>
+  xlet`(POSTv sv. &OPTION_TYPE (LIST_TYPE (LIST_TYPE (SUM_TYPE STRING_TYPE NUM)))
+            (if inFS_fname fs f then
+               SOME(MAP (MAP tokenize_num o tokens blanks) (all_lines fs f))
+             else NONE) sv * STDIO fs)`
+  >- (
+    xapp_spec b_inputAllTokensFrom_spec_specialize >>
+    xsimpl>>
+    fs[FILENAME_def,validArg_def]>>
+    EVAL_TAC)>>
+  pop_assum mp_tac>>
+  TOP_CASE_TAC>>
+  fs[OPTION_TYPE_def]>>
+  strip_tac>>
+  xmatch
+  >- (
+    xlet_autop>>
+    `toks_num = (MAP tokenize_num ∘ tokens blanks)` by
+      metis_tac[toks_num_def,ETA_AX,o_DEF]>>
+    simp[get_graph_def,parse_lad_def]>>
+    TOP_CASE_TAC>>
+    fs[OPTION_TYPE_def]
+    >- (
+      xmatch >>
+      xlet_autop>>
+      xcon>>xsimpl>>
+      qmatch_asmsub_abbrev_tac`STRING_TYPE err _`>>
+      qexists_tac`INL err`>>simp[SUM_TYPE_def])>>
+    xmatch>>
+    xlet_autop>>
+    Cases_on`check_good_graph x`>>xif>>
+    asm_exists_tac>>simp[]
+    >- (
+      xcon>>xsimpl>>
+      qexists_tac`INR x`>>
+      simp[SUM_TYPE_def])>>
+    rpt xlet_autop>>
+    xcon>>xsimpl>>
+    qmatch_asmsub_abbrev_tac`STRING_TYPE err _`>>
+    qexists_tac`INL err`>>simp[SUM_TYPE_def])>>
+  xlet_autop>>
+  xcon>>xsimpl>>
+  qmatch_asmsub_abbrev_tac`STRING_TYPE err _`>>
+  qexists_tac`INL err`>>simp[SUM_TYPE_def]>>
+  fs[get_graph_def]
+QED
 
 (* Translate the encoder *)
 val _ = translate has_mapping_def;
@@ -77,19 +163,172 @@ val _ = translate encode_def;
 (* Translate the string converter *)
 val res = translate enc_string_def;
 
-(* TODO: deduplicate *)
-val r = translate pbc_normaliseTheory.flip_coeffs_def;
-val r = translate pbc_normaliseTheory.pbc_ge_def;
-val r = translate pbc_normaliseTheory.normalise_def;
-
-val r = translate pbc_normaliseTheory.convert_pbf_def;
-val r = translate pbc_normaliseTheory.full_normalise_def;
-
-val res = translate enc_string_def;
-
 val _ = translate full_encode_def;
 
-(* Generic print_pbf *)
+(* parse input from f1 f2 and run encoder *)
+val parse_and_enc = (append_prog o process_topdecs) `
+  fun parse_and_enc f1 f2 =
+  case parse_lad f1 of
+    Inl err => Inl err
+  | Inr pattern =>
+  (case parse_lad f2 of
+    Inl err => Inl err
+  | Inr target =>
+    Inr (full_encode pattern target))`
+
+Theorem parse_and_enc_spec:
+  STRING_TYPE f1 f1v ∧
+  STRING_TYPE f2 f2v ∧
+  validArg f1 ∧
+  validArg f2 ∧
+  hasFreeFD fs
+  ⇒
+  app (p:'ffi ffi_proj) ^(fetch_v"parse_and_enc"(get_ml_prog_state()))
+    [f1v;f2v]
+    (STDIO fs)
+    (POSTv v.
+    STDIO fs *
+    & ∃res.
+     SUM_TYPE STRING_TYPE
+       (LIST_TYPE
+       (PAIR_TYPE PBC_PBOP_TYPE
+          (PAIR_TYPE (LIST_TYPE (PAIR_TYPE INT (PBC_LIT_TYPE STRING_TYPE))) INT))) res v ∧
+      case res of
+        INL err =>
+        get_graph fs f1 = NONE ∨ get_graph fs f2 = NONE
+      | INR pbf =>
+        ∃g1 g2.
+        get_graph fs f1 = SOME g1 ∧
+        get_graph fs f2 = SOME g2 ∧
+        full_encode g1 g2 = pbf)
+Proof
+  rw[]>>
+  xcf"parse_and_enc"(get_ml_prog_state())>>
+  xlet_autop>>
+  Cases_on`res`>>fs[SUM_TYPE_def]>>xmatch
+  >- (
+    xcon>>xsimpl>>
+    qmatch_asmsub_abbrev_tac`STRING_TYPE err _`>>
+    qexists_tac`INL err`>>simp[SUM_TYPE_def])>>
+  xlet_autop>>
+  Cases_on`res`>>fs[SUM_TYPE_def]>>xmatch
+  >- (
+    xcon>>xsimpl>>
+    qmatch_asmsub_abbrev_tac`STRING_TYPE err _`>>
+    qexists_tac`INL err`>>simp[SUM_TYPE_def])>>
+  xlet_autop>>
+  xcon>>
+  xsimpl>>
+  qexists_tac`INR (full_encode y y')`>>
+  simp[SUM_TYPE_def]
+QED
+
+Definition success_string_def:
+  success_string = strlit "Verified pattern graph NOT subgraph isomorphic to target graph\n"
+End
+
+val success_string_v_thm = translate success_string_def;
+
+val check_unsat_3 = (append_prog o process_topdecs) `
+  fun check_unsat_3 f1 f2 f3 =
+  case parse_and_enc f1 f2 of
+    Inl err => TextIO.output TextIO.stdErr err
+  | Inr fml =>
+    (case check_unsat_top success_string fml f3 of
+      Inl err => TextIO.output TextIO.stdErr err
+    | Inr s => TextIO.print s)`
+
+Theorem success_string_not_nil:
+  strlit "" ≠ success_string
+Proof
+  EVAL_TAC
+QED
+
+Definition check_unsat_3_sem_def:
+  check_unsat_3_sem fs f1 f2 out ⇔
+  if out = success_string then
+    ∃pattern target.
+    get_graph fs f1 = SOME pattern ∧
+    get_graph fs f2 = SOME target ∧
+    ¬ has_subgraph_iso pattern target
+  else out = strlit""
+End
+
+Theorem get_graph_good_graph:
+  get_graph fs f = SOME g ⇒
+  good_graph g
+Proof
+  rw[get_graph_def]>>
+  every_case_tac>>
+  fs[]>>
+  metis_tac[check_good_graph,PAIR]
+QED
+
+Theorem check_unsat_3_spec:
+  STRING_TYPE f1 f1v ∧ validArg f1 ∧
+  STRING_TYPE f2 f2v ∧ validArg f2 ∧
+  STRING_TYPE f3 f3v ∧ validArg f3 ∧
+  hasFreeFD fs
+  ⇒
+  app (p:'ffi ffi_proj) ^(fetch_v"check_unsat_3"(get_ml_prog_state()))
+    [f1v; f2v; f3v]
+    (STDIO fs)
+    (POSTv uv. &UNIT_TYPE () uv *
+    SEP_EXISTS out err.
+      STDIO (add_stdout (add_stderr fs err) out) *
+      &(check_unsat_3_sem fs f1 f2 out))
+Proof
+  rw[check_unsat_3_sem_def]>>
+  xcf "check_unsat_3" (get_ml_prog_state ())>>
+  reverse (Cases_on `STD_streams fs`) >- (fs [TextIOProofTheory.STDIO_def] \\ xpull) >>
+  xlet_autop>>
+  Cases_on`res`
+  >- (
+    fs[SUM_TYPE_def]>>
+    xmatch>>
+    xapp_spec output_stderr_spec \\ xsimpl>>
+    asm_exists_tac>>xsimpl>>
+    qexists_tac`emp`>>xsimpl>>
+    qexists_tac`fs`>>xsimpl>>
+    rw[]>>
+    qexists_tac`x`>>
+    xsimpl>>rw[]>>
+    fs[success_string_not_nil,STD_streams_add_stderr, STD_streams_stdout,add_stdo_nil]>>
+    xsimpl)>>
+  fs[SUM_TYPE_def]>>
+  xmatch>>
+  xlet`POSTv v.STDIO fs *
+    SEP_EXISTS res.
+    &(SUM_TYPE STRING_TYPE STRING_TYPE res v ∧
+    ∀s. res = INR s ⇒ s = success_string ∧
+      unsatisfiable (set (full_encode g1 g2)))`
+  >- (
+    xapp>>xsimpl>>
+    rw[]>>fs[pbf_vars_full_encode,success_string_v_thm ]>>
+    fs[FILENAME_def,validArg_def]>>
+    metis_tac[])>>
+  Cases_on`res`>>fs[SUM_TYPE_def]>>xmatch
+  >- (
+    xapp_spec output_stderr_spec \\ xsimpl>>
+    asm_exists_tac>>xsimpl>>
+    qexists_tac`emp`>>xsimpl>>
+    qexists_tac`fs`>>xsimpl>>
+    rw[]>>
+    qexists_tac`strlit ""`>>
+    qexists_tac`x`>>
+    xsimpl>>rw[]>>
+    fs[success_string_not_nil,STD_streams_add_stderr, STD_streams_stdout,add_stdo_nil]>>
+    xsimpl)>>
+  xapp>>asm_exists_tac>>xsimpl>>
+  qexists_tac`emp`>>qexists_tac`fs`>>xsimpl>>
+  rw[]>>
+  qexists_tac`success_string`>>simp[]>>
+  qexists_tac`strlit ""`>>
+  simp[STD_streams_stderr,add_stdo_nil]>>
+  xsimpl>>
+  metis_tac[get_graph_good_graph,full_encode_correct,pbcTheory.unsatisfiable_def]
+QED
+
 Definition print_pbf_def:
   print_pbf f = MAP pbc_string f
 End
@@ -100,104 +339,201 @@ val res = translate pb_parseTheory.op_string_def;
 val res = translate pb_parseTheory.pbc_string_def;
 val res = translate print_pbf_def;
 
-val print_list = (append_prog o process_topdecs) `
-  fun print_list ls =
-    case ls of [] => () | (x::xs) => (print x; print"\n"; print_list xs)`
-
-val parse_and_enc = (append_prog o process_topdecs) `
-  fun parse_and_enc f1 f2 =
-  case parse_lad f1 of
+val check_unsat_2 = (append_prog o process_topdecs) `
+  fun check_unsat_2 f1 f2 =
+    case parse_and_enc f1 f2 of
     Inl err => TextIO.output TextIO.stdErr err
-  | Inr pattern =>
-  (case parse_lad f2 of
-    Inl err => TextIO.output TextIO.stdErr err
-  | Inr target =>
-    full_encode pattern target)
-  `
+  | Inr fml =>
+    TextIO.print_list (print_pbf fml)`
 
-(* TODO: deduplicate *)
-Definition result_string_def:
-  result_string b =
-   if b
-   then INR (strlit "Verified pattern graph NOT subgraph isomorphic to target graph\n")
-   else INL (strlit "Proof checking succeeded but did not derive contradiction\n")
+Definition check_unsat_2_sem_def:
+  check_unsat_2_sem fs f1 f2 out ⇔
+  case get_graph fs f1 of
+    NONE => out = strlit ""
+  | SOME pattern =>
+  case get_graph fs f2 of
+    NONE => out = strlit ""
+  | SOME target =>
+    out = concat (print_pbf (full_encode pattern target))
 End
 
-val r = translate result_string_def;
+Theorem check_unsat_2_spec:
+  STRING_TYPE f1 f1v ∧ validArg f1 ∧
+  STRING_TYPE f2 f2v ∧ validArg f2 ∧
+  hasFreeFD fs
+  ⇒
+  app (p:'ffi ffi_proj) ^(fetch_v"check_unsat_2"(get_ml_prog_state()))
+    [f1v; f2v]
+    (STDIO fs)
+    (POSTv uv. &UNIT_TYPE () uv *
+    SEP_EXISTS out err.
+      STDIO (add_stdout (add_stderr fs err) out) *
+      &(check_unsat_2_sem fs f1 f2 out))
+Proof
+  rw[check_unsat_2_sem_def]>>
+  xcf "check_unsat_2" (get_ml_prog_state ())>>
+  reverse (Cases_on `STD_streams fs`) >- (fs [TextIOProofTheory.STDIO_def] \\ xpull) >>
+  xlet_autop>>
+  Cases_on`res`
+  >- (
+    fs[SUM_TYPE_def]>>
+    every_case_tac>>fs[]>>
+    xmatch>>
+    xapp_spec output_stderr_spec \\ xsimpl>>
+    asm_exists_tac>>xsimpl>>
+    qexists_tac`emp`>>xsimpl>>
+    qexists_tac`fs`>>xsimpl>>
+    rw[]>>
+    qexists_tac`x`>>
+    xsimpl>>rw[]>>
+    fs[success_string_not_nil,STD_streams_add_stderr, STD_streams_stdout,add_stdo_nil]>>
+    xsimpl)>>
+  fs[SUM_TYPE_def]>>
+  xmatch>>
+  xlet_autop>>
+  xapp_spec print_list_spec>>xsimpl>>
+  asm_exists_tac>>xsimpl>>
+  qexists_tac`emp`>>qexists_tac`fs`>>xsimpl>>
+  rw[]>>
+  qexists_tac`strlit ""`>>
+  simp[STD_streams_stderr,add_stdo_nil]>>
+  xsimpl
+QED
 
-val check_unsat' = process_topdecs `
-  fun check_unsat' fml inds id fname =
-  let
-    val fd = TextIO.b_openIn fname
-    val u = (check_header fd;
-      case check_unsat'' fd 1 fml inds id of
-        (fml', (b, (id',inds'))) => result_string b
-      ) handle Fail s => Inl s
-    val close = TextIO.b_closeIn fd;
-  in
-    u
-  end
-  handle TextIO.BadFileName => Inl (notfound_string fname)` |> append_prog;
+Definition usage_string_def:
+  usage_string = strlit "Usage: subgraph_iso_encode <LAD file (pattern)> <LAD file (target)> <optional: proof file>\n"
+End
 
-val _ = translate miscTheory.enumerate_def;
+val r = translate usage_string_def;
 
-val fill_arr = process_topdecs`
-  fun fill_arr arr ls =
-    case ls of [] => arr
-    | (x::xs) =>
-    case x of (i,v) =>
-      fill_arr (Array.updateResize arr None i (Some v)) xs` |> append_prog
-
-(* TODO: Technically, we do not need to run pbc_ge again *)
-val check_unsat_fml = (append_prog o process_topdecs) `
-  fun check_unsat_fml fml fname =
-  let val ls = enumerate 1 (full_normalise fml)
-      val id = List.length ls + 1
-      val arr = Array.array (2*id) None
-      val arr = fill_arr arr ls
-      val inds = []
-  in
-    case check_unsat' arr inds id fname of
-      Inl err => TextIO.output TextIO.stdErr err
-    | Inr s => TextIO.print s
-  end`
-
-val top2 = (append_prog o process_topdecs) `
-  fun top2 f1 f2 =
-  print_list (print_pbf (parse_and_enc f1 f2))`
-
-val top3 = (append_prog o process_topdecs) `
-  fun top3 f1 f2 f3 =
-  let val fml = parse_and_enc f1 f2 in
-    check_unsat_fml fml f3
-  end`
-
-val top = (append_prog o process_topdecs) `
-  fun top u =
+val main = (append_prog o process_topdecs) `
+  fun main u =
   case CommandLine.arguments () of
-    [f1,f2] => top2 f1 f2
-  | [f1,f2,f3] => top3 f1 f2 f3
+    [f1,f2] => check_unsat_2 f1 f2
+  | [f1,f2,f3] => check_unsat_3 f1 f2 f3
   | _ => TextIO.output TextIO.stdErr usage_string`
 
-Theorem top_whole_prog_spec2:
-   hasFreeFD fs ⇒
-   whole_prog_spec2 top_v cl fs NONE (λfs'. ∃err. fs' = foo)
+Definition main_sem_def:
+  main_sem fs cl out =
+  if LENGTH cl = 3 then
+    check_unsat_2_sem fs (EL 1 cl) (EL 2 cl) out
+  else if LENGTH cl = 4 then
+    check_unsat_3_sem fs (EL 1 cl) (EL 2 cl) out
+  else out = strlit ""
+End
+
+Theorem STDIO_refl:
+  (STDIO A ==>> STDIO A) ∧
+  (STDIO A ==>>
+  STDIO A * GC)
 Proof
-  cheat
+  xsimpl
+QED
+
+Theorem main_spec:
+  hasFreeFD fs
+  ⇒
+  app (p:'ffi ffi_proj) ^(fetch_v"main"(get_ml_prog_state()))
+    [Conv NONE []]
+    (COMMANDLINE cl * STDIO fs)
+    (POSTv uv. &UNIT_TYPE () uv *
+    COMMANDLINE cl *
+    SEP_EXISTS out err.
+      STDIO (add_stdout (add_stderr fs err) out) *
+      &(main_sem fs cl out))
+Proof
+  rw[main_sem_def]>>
+  xcf"main"(get_ml_prog_state())>>
+  reverse (Cases_on `STD_streams fs`) >- (fs [TextIOProofTheory.STDIO_def] \\ xpull) >>
+  reverse(Cases_on`wfcl cl`) >- (fs[COMMANDLINE_def] \\ xpull)>>
+  rpt xlet_autop >>
+  Cases_on `cl` >- fs[wfcl_def] >>
+  Cases_on`t`>>fs[LIST_TYPE_def]
+  >- (
+    xmatch>>
+    xapp_spec output_stderr_spec \\ xsimpl>>
+    rename1`COMMANDLINE cl`>>
+    qexists_tac`COMMANDLINE cl`>>xsimpl>>
+    qexists_tac `usage_string` >>
+    simp [theorem "usage_string_v_thm"] >>
+    qexists_tac`fs`>>xsimpl>>
+    rw[]>>
+    fs[success_string_not_nil,STD_streams_add_stderr, STD_streams_stdout,add_stdo_nil]>>
+    metis_tac[STDIO_refl])>>
+  Cases_on`t'`>>fs[LIST_TYPE_def]
+  >- (
+    xmatch>>
+    xapp_spec output_stderr_spec \\ xsimpl>>
+    rename1`COMMANDLINE cl`>>
+    qexists_tac`COMMANDLINE cl`>>xsimpl>>
+    qexists_tac `usage_string` >>
+    simp [theorem "usage_string_v_thm"] >>
+    qexists_tac`fs`>>xsimpl>>
+    rw[]>>
+    fs[success_string_not_nil,STD_streams_add_stderr, STD_streams_stdout,add_stdo_nil]>>
+    metis_tac[STDIO_refl])>>
+  Cases_on`t`>>fs[LIST_TYPE_def]
+  >- (
+    xmatch>>
+    xapp>>fs[]>>
+    rw[]>>
+    fs[wfcl_def]>>
+    first_x_assum (irule_at Any)>>xsimpl>>
+    first_x_assum (irule_at Any)>>xsimpl>>
+    first_x_assum (irule_at Any)>>xsimpl>>
+    rw[]>>
+    metis_tac[STDIO_refl])>>
+  Cases_on`t'`>>fs[LIST_TYPE_def]
+  >- (
+    xmatch>>
+    xapp>>rw[]>>
+    fs[wfcl_def]>>
+    rename1`COMMANDLINE cl`>>
+    qexists_tac`COMMANDLINE cl`>>xsimpl>>
+    rw[]>>metis_tac[STDIO_refl])>>
+  xmatch>>
+  xapp_spec output_stderr_spec \\ xsimpl>>
+  rename1`COMMANDLINE cl`>>
+  qexists_tac`COMMANDLINE cl`>>xsimpl>>
+  qexists_tac `usage_string` >>
+  simp [theorem "usage_string_v_thm"] >>
+  qexists_tac`fs`>>xsimpl>>
+  rw[]>>
+  fs[success_string_not_nil,STD_streams_add_stderr, STD_streams_stdout,add_stdo_nil]>>
+  metis_tac[STDIO_refl]
+QED
+
+Theorem main_whole_prog_spec2:
+   hasFreeFD fs ⇒
+   whole_prog_spec2 main_v cl fs NONE
+     (λfs'. ∃out err.
+        fs' = add_stdout (add_stderr fs err) out ∧
+        main_sem fs cl out)
+Proof
+  rw[basis_ffiTheory.whole_prog_spec2_def]
+  \\ match_mp_tac (MP_CANON (DISCH_ALL (MATCH_MP app_wgframe (UNDISCH main_spec))))
+  \\ xsimpl
+  \\ rw[PULL_EXISTS]
+  \\ qexists_tac`add_stdout (add_stderr fs x') x`
+  \\ xsimpl
+  \\ qexists_tac`x`
+  \\ qexists_tac`x'`
+  \\ xsimpl
+  \\ simp[GSYM add_stdo_with_numchars,with_same_numchars]
 QED
 
 local
 
-val name = "top"
+val name = "main"
 val (sem_thm,prog_tm) =
-  whole_prog_thm (get_ml_prog_state()) name (UNDISCH top_whole_prog_spec2)
-val top_prog_def = Define`top_prog = ^prog_tm`;
+  whole_prog_thm (get_ml_prog_state()) name (UNDISCH main_whole_prog_spec2)
+val main_prog_def = Define`main_prog = ^prog_tm`;
 
 in
 
-Theorem top_semantics =
+Theorem main_semantics =
   sem_thm
-  |> REWRITE_RULE[GSYM top_prog_def]
+  |> REWRITE_RULE[GSYM main_prog_def]
   |> DISCH_ALL
   |> SIMP_RULE(srw_ss())[GSYM CONJ_ASSOC,AND_IMP_INTRO];
 
