examples/pseudo_bool/array/compilation/subgraph_isoCompileScript.sml
@@ -6,6 +6,6 @@ open preamble compilationLib subgraph_isoProgTheory
 val _ = new_theory "subgraph_isoCompile"
 
 val subgraph_iso_compiled = save_thm("subgraph_iso_compiled",
-  compile_x64 "subgraph_iso" top_prog_def);
+  compile_x64 "subgraph_iso" main_prog_def);
 
 val _ = export_theory ();
